commit

MyOCL.thy
@@ -4,10 +4,8 @@ begin
 
 type_synonym var = string
 type_synonym ivar = string
-datatype att = AGE | EMAIL | ID
+datatype att = AGE | EMAIL
 datatype as = LECTURERS | STUDENTS
-
-
 
 datatype OCLexp = Int nat 
   | Var var 
@@ -18,13 +16,16 @@ datatype OCLexp = Int nat
   | Size OCLexp
   | IsEmpty OCLexp
   | Exists OCLexp OCLexp OCLexp
-  | PE OCLexp Objectmodel
+  | Collect OCLexp OCLexp OCLexp
+  (* collect with the body returns a collect-type, then flatten afterwards*)
+  | CollectPlus OCLexp OCLexp OCLexp 
+  | PEAtt OCLexp
+  | PEAs OCLexp "Enrollment list"
   | AllInstances table
 
 fun transAtt :: "MyOCL.att \<Rightarrow> MySQL.col" where
 "transAtt MyOCL.AGE = MySQL.AGE" |
-"transAtt MyOCL.EMAIL = MySQL.EMAIL" |
-"transAtt MyOCL.ID = MySQL.ID" 
+"transAtt MyOCL.EMAIL = MySQL.EMAIL"
 
 fun transAs :: "MyOCL.as \<Rightarrow> MySQL.col" where
 "transAs MyOCL.STUDENTS = MySQL.STUDENTS" |
@@ -39,20 +40,18 @@ fun evalWithCtx :: "OCLexp \<Rightarrow> OCLexp \<Rightarrow> val \<Rightarrow> 
 | "evalWithCtx (MyOCL.Eq e1 e2) var val = 
 VBool (equalVal (evalWithCtx e1 var val) (evalWithCtx e2 var val))" 
 
-
-| "evalWithCtx (PE (MyOCL.Att (Var v) att) om) (MyOCL.IVar i) val
+| "evalWithCtx (PEAtt (MyOCL.Att (Var v) att)) (MyOCL.IVar i) val
 = projVal (Col (transAtt att)) (VObj v)"
 
-| "evalWithCtx (PE (MyOCL.Att (IVar v) att) om) (MyOCL.IVar i) val
+| "evalWithCtx (PEAtt (MyOCL.Att (IVar v) att)) (MyOCL.IVar i) val
 = projVal (Col (transAtt att)) val"
 
+| "evalWithCtx (PEAs (MyOCL.As (Var v) as) es) (MyOCL.IVar i) val
+= VList (extCol (VObj v) (transAs as) es)"
 
-| "evalWithCtx (PE (MyOCL.As (Var v) as) om) (MyOCL.IVar i) val
-= VList (extCol (MySQL.Var v) (transAs as) (getEnrollmentList om))"
+| "evalWithCtx (PEAs (MyOCL.As (IVar v) as) es) (MyOCL.IVar i) val
+= VList (extCol val (transAs as) es)"
 (*
-| "evalWithCtx (PE (MyOCL.As (IVar v) as) om) (MyOCL.IVar i) val
-= VList (extCol (MySQL.IVar v) (transAs as) (getEnrollmentList om))"
-
 | "evalWithCtx (MyOCL.Size exp) var val
 = VList [VInt (sizeVal (evalWithCtx exp var val))]"
 | "evalWithCtx (MyOCL.IsEmpty exp) var val
@@ -72,21 +71,31 @@ fun partialEval :: "OCLexp \<Rightarrow> Objectmodel \<Rightarrow> OCLexp" where
 | "partialEval (MyOCL.Var x) om = (MyOCL.Var x)"
 | "partialEval (MyOCL.IVar i) om = (MyOCL.IVar i)"
 | "partialEval (MyOCL.Eq e1 e2) om = MyOCL.Eq (partialEval e1 om) (partialEval e2 om)" 
-| "partialEval (MyOCL.Att (Var v) att) om = (PE (MyOCL.Att (Var v) att) om)"
-| "partialEval (MyOCL.Att (IVar v) att) om = (PE (MyOCL.Att (IVar v) att) om)"
-| "partialEval (MyOCL.As (Var v) as) om = (PE (MyOCL.As (Var v) as) om)"
-| "partialEval (MyOCL.As (IVar v) as) om = (PE (MyOCL.As (IVar v) as) om)"
+| "partialEval (MyOCL.Att (Var v) att) om = (PEAtt (MyOCL.Att (Var v) att))"
+| "partialEval (MyOCL.Att (IVar v) att) om = (PEAtt (MyOCL.Att (IVar v) att))"
+| "partialEval (MyOCL.As (Var v) as) om = (PEAs (MyOCL.As (Var v) as) (getEnrollmentList om))"
+| "partialEval (MyOCL.As (IVar v) as) om = (PEAs (MyOCL.As (IVar v) as) (getEnrollmentList om))"
+
+fun flatten :: "val list \<Rightarrow> val list" where
+"flatten [] = []" |
+"flatten ((VList vs)#vss) = vs@(flatten vss)"
+
+fun collect :: "val list \<Rightarrow> OCLexp \<Rightarrow> OCLexp \<Rightarrow> val list" where
+"collect [] ivar exp = []"           
+| "collect (val#vs) ivar exp = (evalWithCtx exp ivar val)#(collect vs ivar exp)"
 
 fun eval :: "OCLexp \<Rightarrow> Objectmodel \<Rightarrow> val list" where
 "eval (MyOCL.Int i) om = [VInt i]"
 | "eval (MyOCL.Var x) om = [VObj x]"
 | "eval (MyOCL.Eq e1 e2) om = [VBool (equalValList (eval e1 om) (eval e2 om))]" 
 | "eval (MyOCL.Att (Var v) att) om = projValList (Col (transAtt att)) [VObj v]"
-| "eval (MyOCL.As (Var v) as) om = extCol (MySQL.Var v) (transAs as) (getEnrollmentList om)"
+| "eval (MyOCL.As (Var v) as) om = extCol (VObj v) (transAs as) (getEnrollmentList om)"
 | "eval (MyOCL.Size exp) om = [VInt (sizeValList (eval exp om))]"
 | "eval (MyOCL.IsEmpty exp) om = [VBool (isEmptyValList (eval exp om))]"
 | "eval (MyOCL.Exists src v body) om = [VBool (\<not> isEmptyValList (filterWithBody (eval src om) v (partialEval body om)))]"
 | "eval (MyOCL.AllInstances PERSON) om = mapPersonListToValList (getPersonList om)"
+| "eval (MyOCL.Collect src v body) om = collect (eval src om) v (partialEval body om)"
+| "eval (MyOCL.CollectPlus src v body) om = flatten (collect (eval src om) v (partialEval body om))"
 
 fun translate :: "OCLexp \<Rightarrow> MySQL.exp" where
 "translate (MyOCL.Int i) = MySQL.Int i" |
